mechanization/ErgoC/Lang/ErgoCEval.v
@@ -30,36 +30,37 @@ Require Import ErgoSpec.Common.Utils.Result.
 Require Import ErgoSpec.Common.Utils.Ast.
 
 Require Import ErgoSpec.ErgoC.Lang.ErgoC.
+Require Import ErgoSpec.ErgoC.Lang.ErgoCT.
 Require Import ErgoSpec.ErgoC.Lang.ErgoCEvalContext.
 
 Require Import ErgoSpec.Ergo.Lang.Ergo.
 
-Section ErgoC.
-  Context {h:brand_relation}.
+Section ErgoCTEval.
+  Context {m:brand_model}.
 
-  Definition ergo_unary_eval := ErgoOps.Unary.eval.
-  Definition ergo_binary_eval := ErgoOps.Binary.eval.
+  Definition ergo_unary_builtin_eval := ErgoOps.Unary.eval.
+  Definition ergo_binary_builtin_eval := ErgoOps.Binary.eval.
 
-  Fixpoint ergo_eval_expr (ctxt : eval_context) (expr : ergoc_expr) : eresult ergo_data :=
+  Fixpoint ergoct_eval_expr (ctxt : eval_context) (expr : ergoct_expr) : eresult ergo_data :=
     match expr with
-    | EThisContract prov => contract_in_calculus_error prov
-    | EThisClause   prov => clause_in_calculus_error prov
-    | EThisState    prov => state_in_calculus_error prov
-    | EVar prov name =>
+    | EThisContract (prov,_) => contract_in_calculus_error prov
+    | EThisClause   (prov,_) => clause_in_calculus_error prov
+    | EThisState    (prov,_) => state_in_calculus_error prov
+    | EVar (prov,_) name =>
       match lookup String.string_dec (ctxt.(eval_context_local_env)++ctxt.(eval_context_global_env)) name with
       | None => variable_name_not_found_error prov name
       | Some d => esuccess d
       end
-    | EConst prov d => esuccess d
-    | ENone prov => esuccess dnone
-    | ESome prov e => elift dsome (ergo_eval_expr ctxt e)
-    | EArray prov es =>
+    | EConst (prov,_) d => esuccess d
+    | ENone (prov,_) => esuccess dnone
+    | ESome (prov,_) e => elift dsome (ergoct_eval_expr ctxt e)
+    | EArray (prov,_) es =>
       let rcoll :=
           fold_left
             (fun ls new =>
                match ls with
                | Success _ _ ls' =>
-                 match ergo_eval_expr ctxt new with
+                 match ergoct_eval_expr ctxt new with
                  | Success _ _ new' => esuccess (ls' ++ (new'::nil))
                  | Failure _ _ f => efailure f
                  end
@@ -68,42 +69,46 @@ Section ErgoC.
             es (esuccess nil)
       in
       elift dcoll rcoll
-    | EUnaryOp prov o e  =>
-      match ergo_eval_expr ctxt e with
+    (*** XXX - DISPATCH HERE *)
+    | EBinaryOperator (prov,_) o e1 e2 =>
+      eval_binary_operator_error prov o
+    (*** XXX - DISPATCH HERE *)
+    | EUnaryBuiltin (prov,_) o e  =>
+      match ergoct_eval_expr ctxt e with
       | Success _ _ e' =>
         (* TODO this takes a type hierarchy as a list of string * strings. *)
-        match ergo_unary_eval nil o e' with
+        match ergo_unary_builtin_eval nil o e' with
         | Some r => esuccess r
-        | None => eval_unary_op_error prov o
+        | None => eval_unary_builtin_error prov o
         end
       | Failure _ _ f => efailure f
       end
-    | EBinaryOp prov o e1 e2 =>
-      match ergo_eval_expr ctxt e1 with
+    | EBinaryBuiltin (prov,_) o e1 e2 =>
+      match ergoct_eval_expr ctxt e1 with
       | Success _ _ e1' =>
-        match ergo_eval_expr ctxt e2 with
+        match ergoct_eval_expr ctxt e2 with
         | Success _ _ e2' =>
           (* TODO this takes a type hierarchy as a list of string * strings. *)
-          match ergo_binary_eval nil o e1' e2' with
+          match ergo_binary_builtin_eval nil o e1' e2' with
           | Some r => esuccess r
-          | None => eval_binary_op_error prov o
+          | None => eval_binary_builtin_error prov o
           end
         | Failure _ _ f => efailure f
         end
       | Failure _ _ f => efailure f
       end
-    | EIf prov c t f =>
-      match ergo_eval_expr ctxt c with
-      | Success _ _ (dbool true) => ergo_eval_expr ctxt t
-      | Success _ _ (dbool false) => ergo_eval_expr ctxt f
+    | EIf (prov,_) c t f =>
+      match ergoct_eval_expr ctxt c with
+      | Success _ _ (dbool true) => ergoct_eval_expr ctxt t
+      | Success _ _ (dbool false) => ergoct_eval_expr ctxt f
       | Success _ _ _ => eval_if_not_boolean_error prov
       | Failure _ _ f => efailure f
       end
-    | ELet prov n t v e =>
-      match ergo_eval_expr ctxt v with
+    | ELet (prov,_) n t v e =>
+      match ergoct_eval_expr ctxt v with
       | Success _ _ v' =>
         let ctxt' := eval_context_update_local_env ctxt n v' in
-        ergo_eval_expr ctxt' e
+        ergoct_eval_expr ctxt' e
       | Failure _ _ f => efailure f
       end
     | ERecord prov rs =>
@@ -114,7 +119,7 @@ Section ErgoC.
                let value := snd nv in
                match ls with
                | Success _ _ ls' =>
-                 match ergo_eval_expr ctxt value with
+                 match ergoct_eval_expr ctxt value with
                  (* TODO OpRecConcat to normalize shadowing properly *)
                  | Success _ _ value' => esuccess (ls' ++ ((name, value')::nil))
                  | Failure _ _ f => efailure f
@@ -125,7 +130,7 @@ Section ErgoC.
       in
       elift drec rrec
     (* RIP modularity *)
-    | ENew prov nr rs =>
+    | ENew (prov,_) nr rs =>
       match
         fold_left
           (fun ls nv =>
@@ -133,7 +138,7 @@ Section ErgoC.
              let value := snd nv in
              match ls with
              | Success _ _ ls' =>
-               match ergo_eval_expr ctxt value with
+               match ergoct_eval_expr ctxt value with
                (* TODO OpRecConcat to normalize shadowing properly *)
                | Success _ _ value' => esuccess (ls' ++ ((name, value')::nil))
                | Failure _ _ f => efailure f
@@ -146,9 +151,9 @@ Section ErgoC.
       | Success _ _ r => esuccess (dbrand (nr::nil) (drec r))
       end
     (* EXPECTS: no function calls in expression *)
-    | ECallFun prov fname args => function_not_inlined_error prov "eval" fname
-    | ECallFunInGroup prov gname fname args => function_in_group_not_inlined_error prov gname fname
-    | EMatch prov term pes default =>
+    | ECallFun (prov,_) fname args => function_not_inlined_error prov "eval" fname
+    | ECallFunInGroup (prov,_) gname fname args => function_in_group_not_inlined_error prov gname fname
+    | EMatch (prov,_) term pes default =>
       let lift_dbrand :=
           fun dat brand fn default => 
             match dat with
@@ -160,7 +165,7 @@ Section ErgoC.
             | _ => default
             end
       in
-      match ergo_eval_expr ctxt term with
+      match ergoct_eval_expr ctxt term with
       | Failure _ _ f => efailure f
       | Success _ _ dat =>
         fold_left
@@ -168,25 +173,25 @@ Section ErgoC.
              match pe with
              | (CaseData prov d, res) =>
                if Data.data_eq_dec d dat then
-                 ergo_eval_expr ctxt res
+                 ergoct_eval_expr ctxt res
                else
                  default_result
              | (CaseWildcard prov None, res) =>
-               ergo_eval_expr ctxt res
+               ergoct_eval_expr ctxt res
              | (CaseLet prov name None, res) =>
-               ergo_eval_expr (eval_context_update_local_env ctxt name dat) res
+               ergoct_eval_expr (eval_context_update_local_env ctxt name dat) res
              | (CaseLetOption prov name None, res) =>
                match dat with
-               | dleft dat' => ergo_eval_expr (eval_context_update_local_env ctxt name dat') res
+               | dleft dat' => ergoct_eval_expr (eval_context_update_local_env ctxt name dat') res
                | _ => default_result
                end
              | (CaseWildcard prov (Some typ), res) =>
                lift_dbrand dat typ
-                           (fun dat' => ergo_eval_expr ctxt res)
+                           (fun dat' => ergoct_eval_expr ctxt res)
                            default_result
              | (CaseLet prov name (Some typ), res) =>
                lift_dbrand dat typ
-                           (fun dat' => ergo_eval_expr
+                           (fun dat' => ergoct_eval_expr
                                           (eval_context_update_local_env ctxt name dat')
                                           res)
                            default_result
@@ -194,45 +199,45 @@ Section ErgoC.
                match dat with
                | dleft dat' =>
                 lift_dbrand dat' typ
-                            (fun dat' => ergo_eval_expr
+                            (fun dat' => ergoct_eval_expr
                                             (eval_context_update_local_env ctxt name dat')
                                             res)
                             default_result
                | _ => default_result
                end
              end)
-          pes (ergo_eval_expr ctxt default)
+          pes (ergoct_eval_expr ctxt default)
        end
 
     (* EXPECTS: each foreach has only one dimension and no where *)
-    | EForeach prov ((name,arr)::nil) None fn =>
-      match ergo_eval_expr ctxt arr with
+    | EForeach (prov,_) ((name,arr)::nil) None fn =>
+      match ergoct_eval_expr ctxt arr with
       | Failure _ _ f => efailure f
       | Success _ _ (dcoll arr') =>
         (elift dcoll)
           (emaplift
-             (fun elt => ergo_eval_expr (eval_context_update_local_env ctxt name elt) fn)
+             (fun elt => ergoct_eval_expr (eval_context_update_local_env ctxt name elt) fn)
              arr')
       | Success _ _ _ => eval_foreach_not_on_array_error prov
       end
-    | EForeach prov _ _ _ =>
+    | EForeach (prov,_) _ _ _ =>
       complex_foreach_in_calculus_error prov
     end.
 
-  Definition ergoc_eval_decl
+  Definition ergoct_eval_decl
              (dctxt : eval_context)
-             (decl : ergoc_declaration)
+             (decl : ergoct_declaration)
     : eresult (eval_context * option ergo_data) :=
     match decl with
-    | DCExpr prov expr =>
-      elift (fun x => (dctxt, Some x)) (ergo_eval_expr dctxt expr)
-    | DCConstant prov name ta expr =>
-      let expr' := ergo_eval_expr dctxt expr in
+    | DCTExpr (prov,_) expr =>
+      elift (fun x => (dctxt, Some x)) (ergoct_eval_expr dctxt expr)
+    | DCTConstant (prov,_) name ta expr =>
+      let expr' := ergoct_eval_expr dctxt expr in
       eolift (fun val => esuccess (eval_context_update_global_env dctxt name val, None)) expr'
-    | DCFunc prov name func =>
+    | DCTFunc prov name func =>
       esuccess (dctxt, None)
-    | DCContract prov name contr =>
+    | DCTContract prov name contr =>
       esuccess (dctxt, None)
     end.
 
-End ErgoC.
+End ErgoCTEval.
